new definition of indistinguishability; proof without declassify

coq/two/IndistinguishabilityTwo.v
@@ -16,6 +16,7 @@ Fixpoint atom_LPequiv a1 a2 : Prop :=
       (L = Bottom2 /\ l1 = l2 /\ l1 = Top2 /\
        match v1, v2 with
          | VNat n1, VNat n2 => P v1 v2
+         | VClos e1 t1, VClos e2 t2 => value_LPequiv v1 v2
          | _, _ => True
        end) \/
       (L = Bottom2 /\ l1 = l2 /\ l1 = Bottom2 /\ value_LPequiv v1 v2) \/
@@ -85,7 +86,16 @@ Proof.
       apply Hv in H0. right. left. auto.
     + apply atom_LPequiv_lab_inv in H. inversion H.
     + apply atom_LPequiv_lab_inv in H. inversion H.
-    + destruct v1; destruct v2; left; auto.
+    + destruct v1; destruct v2; left; repeat (split; auto).
+      * assert (t0 = t /\ env_LPequiv Bottom2 P l l0) by
+            (split; destruct H; destruct H; destruct_conjs; subst; auto).
+        destruct_conjs; subst.
+        assert (value_Lequiv Bottom2 (VClos l t) (VClos l0 t)) by
+            (apply Hv; split; auto).
+        assert (env_Lequiv Bottom2 l l0) by
+            (destruct H0; destruct H; destruct_conjs; subst; auto).
+        assumption.
+      * destruct H; destruct H; destruct_conjs; subst; auto.
     + assert (value_LPequiv Top2 P v1 v2) by
           (destruct H; destruct H; destruct_conjs; try inversion H; auto).
       apply Hv in H0. right. right. auto.
@@ -121,3 +131,44 @@ Lemma env_LPequiv_Lequiv :
   forall L P e1 e2,
     env_LPequiv L P e1 e2 -> env_Lequiv L e1 e2.
 Proof. apply atom_value_env_LPequiv_Lequiv. Qed.
+
+Lemma atom_value_env_Top2equiv_Top2Pequiv :
+  forall P,
+    (forall a1 a2,
+       atom_Lequiv Top2 a1 a2 -> atom_LPequiv Top2 P a1 a2)
+    /\ (forall v1 v2,
+          value_Lequiv Top2 v1 v2 -> value_LPequiv Top2 P v1 v2)
+    /\ (forall e1 e2,
+          env_Lequiv Top2 e1 e2 -> env_LPequiv Top2 P e1 e2).
+Proof.
+  intros. apply atom_value_env_mutind.
+  - intros v1 Hv l1 a2 H. destruct a2 as [v2 l2].
+    assert (l2 = l1) by
+        (apply atom_LPequiv_lab_inv in H; subst; auto). 
+    assert (value_LPequiv Top2 P v1 v2) by
+        (apply Hv; destruct H; destruct H; destruct_conjs; inversion H; auto).
+    right. right. auto.
+  - intros n1 v2 H. destruct v2; destruct H; reflexivity.
+  - intros e1 He t1 v2 H. destruct v2 as [n2 | e2 t2]; destruct H; subst.
+    split; try apply He; auto.
+  - intros e1 Ha e2 H. generalize dependent e2.
+    induction e1 as [| a1 e1']; intros; destruct e2 as [| a2 e2']; auto.
+    split; destruct H.
+    + apply (Ha 0); auto.
+    + apply IHe1'; intros; try apply (Ha (S n)); auto.
+Qed.
+
+Lemma atom_Top2equiv_Top2Pequiv :
+  forall P a1 a2,
+    atom_Lequiv Top2 a1 a2 -> atom_LPequiv Top2 P a1 a2.
+Proof. apply atom_value_env_Top2equiv_Top2Pequiv. Qed.
+
+Lemma value_Top2equiv_Top2Pequiv :
+  forall P v1 v2,
+    value_Lequiv Top2 v1 v2 -> value_LPequiv Top2 P v1 v2.
+Proof. apply atom_value_env_Top2equiv_Top2Pequiv. Qed.
+
+Lemma env_Top2equiv_Top2Pequiv :
+  forall P e1 e2,
+    env_Lequiv Top2 e1 e2 -> env_LPequiv Top2 P e1 e2.
+Proof. apply atom_value_env_Top2equiv_Top2Pequiv. Qed.
