coq/two/LambdaTwo.v
@@ -1,30 +1,48 @@
 Require Export LambdaTwoSyntax.
 Require Export IndistinguishabilityTwo.
 
-(** * Its semantics: big step evaluation judgment. *)
-Reserved Notation "P , pc ; e ⊢ t ⇓ a" (at level 70).
+Reserved Notation "[ L , P , k ] pc ; e ⊢ t ⇓ a" (at level 70).
 Inductive eval :
-  (value -> value -> Prop) -> two -> env -> term -> atom -> Prop :=
-| E_Nat : forall P pc e n,
-(* ------------------------------------- *)
-    P, pc; e ⊢ TNat n ⇓ Atom (VNat n) pc
-| E_Var : forall P pc e n v l,
+  two -> (value -> value -> Prop) -> nat ->
+  two -> env -> term -> atom -> Prop :=
+
+| E_Nat : forall L P k pc e n,
+(* ------------------------------------------------------ *)
+    [L, P, k] pc; e ⊢ TNat n ⇓ Atom (VNat n) pc
+
+| E_Var : forall L P k pc e n v l,
     atIndex e n = Some (Atom v l) ->
-(* ---------------------------------- *)
-    P, pc; e ⊢ TVar n ⇓ Atom v (l ⊔ pc)
-| E_Abs : forall P pc e t,
-(* -------------------------------------- *)
-    P, pc; e ⊢ TLam t ⇓ Atom (VClos e t) pc
-| E_App : forall P pc e t1 t2 e1' t1' l1 a2 a3,
-    P, pc; e ⊢ t1 ⇓ Atom (VClos e1' t1') l1 ->
-    P, pc; e ⊢ t2 ⇓ a2 ->
-    P, l1; a2 :: e1' ⊢ t1' ⇓ a3 ->
-(* ----------------------------------------- *)
-    P, pc; e ⊢ TApp t1 t2 ⇓ a3
-| E_Decl1 : forall P pc e t1 t2 v,
-    P, pc; e ⊢ TApp t1 t2 ⇓ Atom v Bottom2 ->
-(* ----------------------------------------- *)
-    P, pc; e ⊢ TDecl t1 t2 ⇓ Atom v Bottom2
-where "P , pc ; e ⊢ t ⇓ a" := (eval P pc e t a).
+(* ------------------------------------------------------ *)
+    [L, P, k] pc; e ⊢ TVar n ⇓ Atom v (l ⊔ pc)
+
+| E_Abs : forall L P k pc e t,
+(* ------------------------------------------------------ *)
+    [L, P, k] pc; e ⊢ TLam t ⇓ Atom (VClos e t) pc
+
+| E_App : forall L P k pc e t1 t2 e1' t1' l1 a2 a3,
+    [L, P, k] pc; e ⊢ t1 ⇓ Atom (VClos e1' t1') l1 ->
+    [L, P, k] pc; e ⊢ t2 ⇓ a2 ->
+    [L, P, k] l1; a2 :: e1' ⊢ t1' ⇓ a3 ->
+(* ------------------------------------------------------ *)
+    [L, P, k] pc; e ⊢ TApp t1 t2 ⇓ a3
+
+| E_Decl1 : forall L P k pc e t1 t2 v,
+    [L, P, k] pc; e ⊢ TApp t1 t2 ⇓ Atom v Bottom2 ->
+(* ------------------------------------------------------ *)
+    [L, P, k] pc; e ⊢ TDecl t1 t2 ⇓ Atom v Bottom2
+
+(*| E_Decl2 : forall L P k pc e t1 t2 e1' t1' l1 a2 v3,
+    [L, P, k] pc; e ⊢ t1 ⇓ Atom (VClos e1' t1') l1 ->
+    [L, P, k] pc; e ⊢ t2 ⇓ a2 ->
+    [L, P, k] l1; a2 :: e1' ⊢ t1' ⇓ Atom v3 Top2 ->
+    (forall a a' v v',
+       atom_LPequiv L P a a' ->
+       [L, P, k] l1; a :: e1' ⊢ t1' ⇓ Atom v Top2 ->
+       [L, P, k] l1; a' :: e1' ⊢ t1' ⇓ Atom v' Top2 ->
+       value_Lequiv L v v') ->
+(* ------------------------------------------------------ *)
+    [L, P, (S k)] pc; e ⊢ TDecl t1 t2 ⇓ Atom v3 Bottom2*)
+
+where "[ L , P , k ] pc ; e ⊢ t ⇓ a" := (eval L P k pc e t a).
 
 Hint Constructors eval.
