coq/two/LambdaTwoNI.v
@@ -3,98 +3,60 @@ Require Import LambdaTwo.
 
 Section NI.
 
-Lemma non_interference_top :
-  forall (P : value -> value -> Prop) pc e1 e2 t a1 a2,
+Lemma non_interference :
+  forall L (P : value -> value -> Prop) k pc e1 e2 t a1 a2,
     (forall x, P x x) ->
-    env_Lequiv Top2 e1 e2 ->
-    P, pc; e1 ⊢ t ⇓ a1 ->
-    P, pc; e2 ⊢ t ⇓ a2 ->
-    atom_Lequiv Top2 a1 a2.
+    env_LPequiv L P e1 e2 ->
+    [L, P, k] pc; e1 ⊢ t ⇓ a1 ->
+    [L, P, k] pc; e2 ⊢ t ⇓ a2 ->
+    atom_LPequiv L P a1 a2.
 Proof.
-  intros P pc e1 e2 t a1 a2 Prefl He Heval.
+  intros L P k pc e1 e2 t a1 a2 Prefl He Heval.
   generalize dependent a2.
   generalize dependent e2.
-  induction Heval; intros e2 He a3' Heval2'; inversion Heval2'; subst.
-  - (* E_Nat *)
-    destruct pc; right; right; auto.
-  - (* E_Var *)
-    rename e into e1.
+  induction Heval; intros e2 He a3' Heval2';
+  inversion Heval2'; rename e into e1; subst.
+  - (* E_Nat *) 
+    destruct L; destruct pc.
+    + right. left. auto.
+    + left. auto.
+    + right. right. auto.
+    + right. right. auto.
+  - (* E_Var *) 
     rename v into v1. rename l into l1.
     rename v0 into v2. rename l0 into l2.
-    unfold env_Lequiv in He. unfold env_LPequiv in He.
-    assert (atom_Lequiv Top2 (Atom v1 l1) (Atom v2 l2)) by
-        (eapply list_forall2_atIndex; eassumption).
-    assert (l2 = l1) by
-        (unfold atom_Lequiv in H0; apply atom_LPequiv_lab_inv in H0;
-         subst; reflexivity). subst.
-    destruct pc; unfold atom_Lequiv in H0.
-    + rewrite join_bot. eapply atom_LPequiv_Lequiv. eassumption.
-    + rewrite join_top. destruct l1; auto.
-      eapply atom_LPequiv_raise; eauto.
-  - (* E_Abs *)
-    rename e into e1. 
-    unfold env_Lequiv in He. 
-    apply env_LPequiv_Lequiv in He.
-    destruct pc; right; right; auto.
+    destruct pc.
+    + rewrite 2! join_bot in *.
+      eapply list_forall2_atIndex in H6; eauto.
+    + rewrite 2! join_top in *.
+      assert (atom_LPequiv L P (Atom v1 l1) (Atom v2 l2)) by
+          (eapply list_forall2_atIndex; eassumption).
+      assert (l2 = l1) by
+          (apply atom_LPequiv_lab_inv in H0; subst; reflexivity).
+      destruct l1; subst; auto.
+      apply atom_LPequiv_raise; auto.
+  - (* E_Abs *) 
+    destruct L; destruct pc.
+    + right. left. auto.
+    + left. auto.
+    + right. right. auto.
+    + right. right. auto.
   - (* E_App *)
-    rename e into e1. rename a0 into a2'.
+    rename a0 into a2'.
     rename e1'0 into e2'. rename t1'0 into t2'. rename l0 into l2.
     destruct a3 as [v3 l3]; destruct a3' as [v3' l3'].
     apply IHHeval1 in H1.
-    apply IHHeval2 in H5. {
+    apply IHHeval2 in H7. {
       assert (l2 = l1) by
           (apply atom_LPequiv_lab_inv in H1; subst; reflexivity). subst.
-      destruct l1;
-        assert (t2' = t1' /\ env_Lequiv Top2 e1' e2') by
-          (split; destruct H1; destruct H; destruct_conjs; inversion H; auto);
-        destruct_conjs; subst;
-        eapply IHHeval3; eauto; split; assumption.
+      assert (t2' = t1' /\ env_LPequiv L P e1' e2') by
+          (split; destruct H1; destruct H; destruct_conjs;
+           try inversion H1; subst; auto).
+      destruct_conjs; subst. eapply IHHeval3; eauto. split; assumption.
     } assumption. assumption. assumption. assumption.
   - (* E_Decl1 *)
-    rename v into v1. rename v0 into v2. rename e into e1.
+    rename v into v1. rename v0 into v2. 
     eapply IHHeval; eauto.
 Qed.
-
-Lemma non_interference_bot :
-  forall (P : value -> value -> Prop) pc e1 e2 t a1 a2,
-    (forall x, P x x) ->
-    env_LPequiv Bottom2 P e1 e2 ->
-    P, pc; e1 ⊢ t ⇓ a1 ->
-    P, pc; e2 ⊢ t ⇓ a2 ->
-    atom_Lequiv Bottom2 a1 a2.
-Proof.
-  intros P pc e1 e2 t a1 a2 Prefl He Heval.
-  generalize dependent a2.
-  generalize dependent e2.
-  induction Heval; intros e2 He a3' Heval2'; inversion Heval2'; subst.
-  - (* E_Nat *)
-    destruct pc; [right; left; auto | left; auto].
-  - (* E_Var *)
-    rename e into e1.
-    rename v into v1. rename l into l1.
-    rename v0 into v2. rename l0 into l2.
-    unfold env_LPequiv in He.
-    assert (atom_LPequiv Bottom2 P (Atom v1 l1) (Atom v2 l2)) by
-        (eapply list_forall2_atIndex; eassumption).
-    assert (l2 = l1) by
-        (apply atom_LPequiv_lab_inv in H0; subst; reflexivity). subst.
-    destruct pc.
-    + rewrite join_bot. eapply atom_LPequiv_Lequiv. eassumption.
-    + rewrite join_top. destruct l1.
-      * apply atom_LPequiv_raise in H0.
-          eapply atom_LPequiv_Lequiv. eassumption.
-        assumption.
-      * eapply atom_LPequiv_Lequiv. eassumption.
-  - (* E_Abs *)
-    rename e into e1.
-    apply env_LPequiv_Lequiv in He.
-    destruct pc; [right; left; auto | left; auto].
-  - (* E_App *)
-    admit.
-  - (* E_Decl1 *)
-    rename e into e1.
-    rename v into v1. rename v0 into v2.
-    eapply IHHeval; eauto.
-Qed.
-
+  
 End NI.
